Dataflow/Syntax.v
@@ -14,23 +14,23 @@ Implicit Type ck : clock.
 
 (** ** Syntax *)
 
-Inductive lexp : Type :=
+Inductive lexp : Set :=
   | Econst : const -> lexp
   | Evar : ident -> lexp
   | Ewhen : lexp -> ident -> bool -> lexp
   | Eop : operator -> list lexp -> lexp.
 
-Inductive laexp : Type :=
+Inductive laexp : Set :=
   | LAexp : clock -> lexp -> laexp.
 
 Implicit Type le: lexp.
 Implicit Type lae: laexp.
 
-Inductive cexp : Type :=
+Inductive cexp : Set :=
   | Emerge : ident -> cexp -> cexp -> cexp 
   | Eexp : lexp -> cexp.
 
-Inductive caexp : Type :=
+Inductive caexp : Set :=
   | CAexp : clock -> cexp -> caexp.
 
 Implicit Type ce: cexp.
@@ -38,7 +38,7 @@ Implicit Type cae: caexp.
 
 (** ** Equations *)
 
-Inductive equation : Type :=
+Inductive equation : Set :=
   | EqDef : ident -> caexp -> equation
   | EqApp : ident -> ident -> laexp -> equation
   | EqFby : ident -> const -> laexp -> equation.
@@ -47,7 +47,7 @@ Implicit Type eqn: equation.
 
 (** ** Node *)
 
-Record node : Type := mk_node {
+Record node : Set := mk_node {
   n_name : ident;
   n_input : ident;
   n_output : ident;
@@ -66,3 +66,21 @@ Definition find_node (f : ident) : global -> option node :=
   List.find (fun n=> ident_eqb n.(n_name) f).
 
 
+(** Stronger induction scheme for lexp *)
+Definition lexp_ind2 : forall P : lexp -> Prop,
+  (forall c, P (Econst c)) ->
+  (forall i, P (Evar i)) ->
+  (forall le, P le -> forall i b, P (Ewhen le i b)) ->
+  (forall op les, List.Forall P les -> P (Eop op les)) ->
+  forall le, P le.
+Proof.
+intros P Hconst Hvar Hwhen Hop. fix 1.
+intro le.
+destruct le as [c | i | le | op les].
++ apply Hconst.
++ apply Hvar.
++ apply Hwhen. apply lexp_ind2.
++ apply Hop. induction les; constructor.
+  - apply lexp_ind2.
+  - apply IHles.
+Defined.
